
\documentclass{package/notes}
\usepackage[english]{babel}
\usepackage{amssymb,amsmath,amsfonts}  %%% for maths
%%%%%%%%%%%%%%%%%%%%%%%%%%%%%%%%%%%%%
\usepackage{package/color-env}
\usepackage{lipsum}
\renewcommand\qedsymbol{$\blacksquare$}
%%%%%%%%%%%%%%%%%%%%%%%%%%%%%%%%%%%%%

\begin{document}

\textbf{Question 1:} Solve the following system of differential equations:

\begin{equation*}
	\begin{aligned}
		y_1'(t) =&\: 5y_1(t) - 7y_2(t)\\
		y_2'(t) =&\: 2y_1(t) - 4y_2(t)
	\end{aligned}
\end{equation*}\\

\textbf{Step \#1: Create a matrix equation comprising of the two differential equations:}

\begin{equation*}
	\begin{aligned}
		\mathbf{y'} =&\: A\mathbf{y}\\
		\left[\begin{array}{c}
			y_1'(t) \\ y_2'(t)
		\end{array}\right] =&\: 
		\left[\begin{array}{cc}
			-5 & -7\\ -2 & -4
		\end{array}\right]
		\left[\begin{array}{c}
			y_1(t) \\ y_2(t)
	\end{array}\right]
	\end{aligned}
\end{equation*}

\textbf{Step \#2: Calculate the determinant}\\

\textbf{Step \#3: For each eigenvalue, calculate the eigenvectors:}\\

In order to find the associated eigenvectors, we simply substitute $\lambda$ \\into $(A-I\lambda) = \vec 0$

\textbf{Step \#4: }\\
\textbf{Step \#5: Calculate the general solution:}\\
\textbf{Step \#6: Given initial conditions $\mathbf{y} = \left[\begin{array}{c}16\\6\end{array}\right]$ solve for $c_1$ and $c_2$ to find the specific solution}

\begin{equation*}
	\begin{aligned}
		16 =&\: 7c_1 + c_2\\
		6 =&\: 2c_1 + c_2\\
		(16-6) =&\: (7c_1-2c_2) + (c_2-c_2)\\
		10 =&\: 5c_1\\
		c_1 =&\: 2\\\\
		6 =&\: 2(2) + c_2\\
		6 =&\: 4 + c_2\\
		2 =&\: c_2
	\end{aligned}
\end{equation*}

\textbf{Step \#7: State the answer}

Way \#1: Express as a system of equations:

\begin{equation*}
	\begin{aligned}
		y_1(t) =&\: 14e^{3t} + 2e^{-2t}\\
		y_2(t) = &\: 4e^{3t} + 2e^{-2t}\\
	\end{aligned}
\end{equation*}\\

Way \#2: Express as an array:

\begin{equation*}
	\begin{aligned}
		\left[\begin{array}{c} y_1(t) \\ y_2(t) \end{array}\right] 
		= 2\left[\begin{array}{c} 7e^{3t} \\ 2e^{3t}\end{array}\right] 
		+ 2\left[\begin{array}{c} e^{-2t}\\e^{-2t}\end{array}\right]
	\end{aligned}
\end{equation*}




\end{document}
.